feat: translate Relations and STLC example proof
Experimented with the form of the main proof using a simpler STLC with named variables and types in the AST.

Created Inductive TranslatesTo relations from this STLC and from the STLC  subset of Lambda Box T to PIR. Using reflect proofs, this can be used to generate the necessary lemma's through inversion (instead of writing them by hand)

theories/Semantics.v
@@ -1,157 +1,142 @@
 From MetaCoq.Erasure.Typed Require Import ExAst Utils WcbvEvalAux.
 From MetaCoq.Erasure.Typed Require Import TypeAnnotations.
 From MetaCoq.Erasure.Typed Require Import Annotations.
-From MetaCoq.Erasure Require Import EAst EWellformed.
+From MetaCoq.Erasure Require Import EAst ECSubst EWellformed.
 From MetaCoq.Utils Require Import utils.
 
 From VTL Require Import PIR BigStepPIR Translation.
 
 Existing Instance EWcbvEval.default_wcbv_flags.
 
-Inductive InReflSubset (ctx : context) : EAst.term -> Prop :=
+(* do we need context? *)
+Inductive InReflSubset (ctx : list bs) : EAst.term -> Prop :=
   | RS_tBox : InReflSubset ctx tBox
   | RS_tRel : forall n res,
     nth_error ctx n = Some res ->
     InReflSubset ctx (tRel n)
-  | RS_tLambda : forall na t,
-    InReflSubset ctx t ->
-    InReflSubset ctx (tLambda na t)
+  | RS_tLambda : forall na b,
+    InReflSubset ctx b ->
+    InReflSubset ctx (tLambda na b)
 .
 
-Inductive InSubset (ctx : context) : EAst.term -> Prop :=
+Inductive InSubset (ctx : list bs) : EAst.term -> Prop :=
   | S_tBox : InSubset ctx tBox
   | S_tRel : forall n res,
     nth_error ctx n = Some res ->
     InSubset ctx (tRel n)
-  | S_tLambda : forall na t,
-    InSubset ctx t ->
-    InSubset ctx (tLambda na t)
+  | S_tLambda : forall na b,
+    InSubset ctx b ->
+    InSubset ctx (tLambda na b)
   | S_tApp : forall t1 t2,
     InSubset ctx t1 ->
     InSubset ctx t2 ->
     InSubset ctx (tApp t1 t2)
 .
 
-Definition gal_id :=
-  tLambda (BasicAst.nNamed "x") (tRel 0).
-
 Import Coq.Strings.String.
 Local Open Scope string_scope.
+Import MCMonadNotation.
 
-Notation "ctx p⊢ tl{ gt | ann_gt }" := (translate_term remap_env ctx gt ann_gt) (at level 100).
-Notation "ctx p⊢ { gt | ann_gt } '⇓ₚ' { gv | ann_gv }" :=
-  (forall pt pv,
-  (translate_term remap_env ctx gt ann_gt) = Some pt ->
-  (translate_term remap_env ctx gv ann_gv) = Some pv ->
-  (evaluatesTo pt pv))
-  (at level 50, gt, ann_gt, gv, ann_gv at next level).
+Notation "ctx ⊢ tl{ gt | ann_gt }" := (translate_term remap_env ctx gt ann_gt) (at level 100).
+Notation "pt '⇓ₚ' pv" :=
+  (evaluatesTo pt pv)
+  (at level 50).
 
 Ltac solve_pir_eval := split; [(eexists ; eauto using eval) | constructor].
-Ltac solve_inv_eval := intros pt pv Hgt Hgv; inversion Hgt; inversion Hgv; solve_pir_eval.
+Ltac solve_inv := intros pt pv Hgt Hgv; inversion Hgt; inversion Hgv; solve_pir_eval.
 Ltac solve_err := simpl in *; try contradiction; try discriminate.
 
-Lemma galEvalId : forall Σ, Σ e⊢ gal_id ⇓ gal_id.
-Proof.
-  intros. eauto.
-Qed.
+Definition gal_id :=
+  tLambda (BasicAst.nNamed "x"%bs) (tRel 0).
 
-Theorem id_correct_explicit : forall Σ, 
+Theorem id_correct_explicit : forall Σ ctx pir_id, 
   let ann := (TArr (TConst <%% unit %%>) (TConst <%% unit %%>), (TConst <%% unit %%>)) in
   Σ e⊢ gal_id ⇓ gal_id ->
-  nil p⊢ {gal_id | ann} ⇓ₚ {gal_id | ann}.
+  (translate_term remap_env ctx gal_id ann) = Some pir_id ->
+  pir_id ⇓ₚ pir_id.
 Proof with (eauto using eval).
-  intros Σ ann ev.
+  intros Σ ctx pir_id ann ev tl.
   unfold gal_id in *. simpl in *.
-  solve_inv_eval.
+  inversion tl. solve_pir_eval.
 Qed.
 
-Theorem id_correct_implicit : forall Σ ctx (ann : annots box_type gal_id),
+Theorem id_correct_implicit : forall Σ ctx (ann : annots box_type gal_id) pir_id,
   Σ e⊢ gal_id ⇓ gal_id ->
-  InSubset ctx gal_id ->
-  ctx p⊢ { gal_id | ann } ⇓ₚ { gal_id | ann }.
+  (translate_term remap_env ctx gal_id ann) = Some pir_id ->
+  pir_id ⇓ₚ pir_id.
 Proof with (eauto using eval).
-  intros Σ ctx ann ev sub.
+  intros Σ ctx ann pir_id ev tl.
   unfold gal_id in *.
-  destruct ann as [bt a]. rewrite unfold_lamAbs.
-  destruct (decompose_arr bt) as [[] _]; try discriminate.
-  destruct (get_type remap_env b). simpl.
-  - solve_inv_eval.
-  - discriminate.
+  destruct ann as [ty t_ty]. rewrite unfold_lamAbs in tl.
+  destruct ty; try discriminate.
+  destruct (translate_ty remap_env ty1);
+  inversion tl; solve_pir_eval.
 Qed.
 
-Theorem tl_lambda : forall ctx na t (ann : annots box_type (tLambda na t)),
-  ctx p⊢ { tLambda na t | ann} ⇓ₚ { tLambda na t | ann}.
-Proof with (eauto using eval).
-  intros ctx na t ann.
-  destruct ann as [bt a]. rewrite unfold_lamAbs.
-  destruct (decompose_arr bt) as [[] _]; try discriminate.
-  destruct (get_type remap_env b) as [ty|]; try discriminate.
-  destruct t; try discriminate; simpl.
-  - solve_inv_eval.
-  - destruct (nth_error (vass (BasicAst.nNamed (s_to_bs get_name na)) :: ctx) n).
-    destruct c. destruct decl_name; try discriminate. simpl.
-    + solve_inv_eval.
-    + discriminate.
-  - destruct a as [[] a']; try discriminate.
-    + simpl. destruct (decompose_arr codom).
-    destruct (get_type remap_env dom) as [ty'|]; try discriminate. admit.
-  - admit.
-Admitted.
-
-(* use unfold lemmas, translate app = *)
-Theorem refl_tl_correct : forall Σ ctx gt (ann : annots box_type gt),
+(* contexts don't match in both branches! *)
+Lemma tl_app : forall ctx t1 t2 ann_t (t' : PIR.term),
+  translate_term remap_env ctx (tApp t1 t2) ann_t = Some t' ->
+  exists ann_t1 ann_t2 t1' t2',
+    translate_term remap_env ctx t1 ann_t1 = Some t1' /\
+    translate_term remap_env ctx t2 ann_t2 = Some t2' /\
+    Apply t1' t2' = t'.
+Proof.
+  intros ctx t1 t2 ann_t t' tl_a.
+  inversion tl_a as [Ha].
+  destruct ann_t as [ann_t [ann_t1 ann_t2]].
+  destruct (translate_term remap_env ctx t1 ann_t1) as [t1'|] eqn:Et1; try discriminate.
+  destruct (translate_term remap_env ctx t2 ann_t2) as [t2'|] eqn:Et2; try discriminate. 
+  simpl in Ha. exists ann_t1. exists ann_t2. exists t1'. exists t2'.
+  inversion Ha. auto.
+Qed.
+  
+Theorem refl_tl_correct : forall Σ ctx gt (ann : annots box_type gt) pt,
   Σ e⊢ gt ⇓ gt ->
   InReflSubset ctx gt ->
-  ctx p⊢ { gt | ann} ⇓ₚ {gt | ann}.
+  (translate_term remap_env ctx gt ann) = Some pt ->
+  pt ⇓ₚ pt.
 Proof with (eauto using eval).
-  intros Σ ctx gt ann ev rsub.
+  intros Σ ctx gt ann pt ev rsub tl.
   destruct rsub.
-  - (* TBox *) solve_inv_eval.
-  - (* tRel, either an error or ev is invalid *) 
-    simpl in *. destruct (nth_error ctx n). destruct c. destruct decl_name.
-    + discriminate.
-    + now inversion ev.
-    + discriminate.
-  - (* tLambda *) destruct ann as [bt a]. rewrite unfold_lamAbs.
-  destruct (decompose_arr bt). destruct l; try discriminate.
-  destruct (get_type remap_env b0) as [ty|]; try discriminate.
-  destruct ty eqn:Ety; simpl; try discriminate. admit.
+  - (* TBox *) inversion tl. solve_pir_eval.
+  - (* tRel, either a translation error or ev is invalid *) 
+    now inversion ev.
+  - (* tLambda *) destruct ann as [ty t_ty]; try discriminate. 
+    destruct na.
+    + solve_err. 
+    + simpl in tl. destruct ty; try discriminate.
+      destruct (translate_ty remap_env ty1) as [ty1'|]; try discriminate.
+      destruct (i :: ctx ⊢ tl{ b | t_ty}) as [b'|]; try discriminate.
+      inversion tl. solve_pir_eval.
 Qed.
 
-(*Definition id_app := tApp
+(* subst lemma, or use the named variant of EAst *)
+(* Print csubst. *)
+Lemma tl_subst : forall ctx k x v b ann_v ann_b ann_t v' b',
+  translatesTo remap_env ctx v ann_v v' ->
+  translatesTo remap_env ctx b ann_b b' ->
+  translatesTo remap_env ctx (csubst v k b) ann_t (BigStepPIR.subst x v' b').
+Proof.
+  intros ctx k x v b ann_v ann_b ann_t v' b' tlt_v tlt_b.
+  inversion tlt_b.
+  - simpl. subst. apply tlt_tt.
+  - simpl in *. destruct (x =? (bs_to_s x0)). subst.
+    simpl in *. inversion tlt_v. Admitted.
+
+
+Definition id_app := tApp
   (tLambda (BasicAst.nNamed "x"%bs) (tRel 0)) (tBox).
 
-Theorem id_app_correct : forall ctx (ann : annots box_type id_app),
-  ~ (ctx p⊢ tl_err{id_app | ann}) ->
-  ctx p⊢ {id_app | ann} ⇓ₚ {tBox | TBox}.
-Proof with (eauto using eval).
-  intros ctx ann nerr.
-  unfold id_app. destruct ann. destruct p. rewrite unfold_app. split.
-  - eexists. eapply E_Apply... 
-  (* destruct ann as [annv [[dom codom] bt]]; try solve_err.
-  destruct (decompose_arr dom); destruct l; try solve_err.
-  unfold not in nerr. simpl in nerr. destruct nerr. left. trivial.
-  destruct (get_type remap_env b0); split. 
-  - eexists. eapply E_Apply... simpl...
-  - constructor.
-  - eexists. admit. (* it sees λ(x : tt, x) x as valid*)
-  - constructor.
-  - unfold not in nerr. simpl in nerr. destruct nerr. left. trivial.
-  - constructor. *)
-Admitted.
-
 Theorem stlc_correct : forall Σ ctx 
-  gt (ann_gt : annots box_type gt)
-  gv (ann_gv : annots box_type gv),
+  gt (ann_gt : annots box_type gt) pt
+  gv (ann_gv : annots box_type gv) pv,
   Σ e⊢ gt ⇓ gv ->
   InSubset ctx gt ->
-  ~ (ctx p⊢ tl_err{gt | ann_gt}) ->
+  translate_term remap_env ctx gt ann_gt = Some pt ->
   InSubset ctx gv ->
-  ~ (ctx p⊢ tl_err{gv | ann_gv}) ->
-  ctx p⊢ {gt | ann_gt} ⇓ₚ {gv | ann_gv}.
+  translate_term remap_env ctx gv ann_gv = Some pv ->
+  pt ⇓ₚ pv.
 Proof with (eauto using eval).
-  intros Σ ctx gt ann_gt gv ann_gv.
-  intros ev sub_gt nerr_gt sub_gv nerr_gv.
-  (* main proof, set up useful lemmas first *)
-  (* refl cases*)
-Admitted. *)
+  intros Σ ctx gt ann_gt pt gv ann_gv pv ev sub_gt.
+  revert pt pv. induction ev; try discriminate; intros pt pv.
+  - simpl. destruct ann_gt. Admitted.
