theories/Stlc.v
@@ -7,7 +7,8 @@ Module STLC.
 
 Inductive ty : Type :=
   | Ty_Bool  : ty
-  | Ty_Arrow : ty -> ty -> ty.
+  | Ty_Arrow : ty -> ty -> ty
+  | Ty_ERROR : ty.
 
 Definition context := env ty.
 
@@ -16,7 +17,8 @@ Inductive tm : Type :=
   | tm_app   : tm -> tm -> tm
   | tm_abs   : string -> ty -> tm -> tm
   | tm_true  : tm
-  | tm_false : tm.
+  | tm_false : tm
+  | tm_oops  : tm.
   (* | tm_if    : tm -> tm -> tm -> tm. *)
 
 Declare Scope stlc_scope.
@@ -31,7 +33,7 @@ Notation "x" := x (in custom stlc_ty at level 0, x global) : stlc_scope.
 Notation "<{{ x }}>" := x (x custom stlc_ty).
 
 Notation "( t )" := t (in custom stlc_ty at level 0, t custom stlc_ty) : stlc_scope.
-Notation "S -> T" := (Ty_Arrow S T) (in custom stlc_ty at level 99, right associativity) : stlc_scope.
+Notation "ty1 -> ty2" := (Ty_Arrow ty1 ty2) (in custom stlc_ty at level 99, right associativity) : stlc_scope.
 
 Notation "$( t )" := t (in custom stlc_ty at level 0, t constr) : stlc_scope.
 
@@ -44,8 +46,9 @@ Notation "'Bool'" := Ty_Bool (in custom stlc_ty at level 0) : stlc_scope.
                     left associativity). *)
 Notation "'true'"  := true (at level 1).
 Notation "'true'"  := tm_true (in custom stlc_tm at level 0).
-Notation "'false'"  := false (at level 1).
-Notation "'false'"  := tm_false (in custom stlc_tm at level 0).
+Notation "'false'" := false (at level 1).
+Notation "'false'" := tm_false (in custom stlc_tm at level 0).
+Notation "'OOPS'" := tm_oops (in custom stlc_tm at level 0).
 
 Notation "$( x )" := x (in custom stlc_tm at level 0, x constr, only parsing) : stlc_scope.
 Notation "x" := x (in custom stlc_tm at level 0, x constr at level 0) : stlc_scope.
@@ -69,8 +72,8 @@ Hint Unfold y : core.
 Hint Unfold z : core.
 
 Inductive value : tm -> Prop :=
-  | v_abs : forall x T2 t1,
-      value <{\x:T2, t1}>
+  | v_abs : forall x ty2 t1,
+      value <{\x:ty2, t1}>
   | v_true :
       value <{true}>
   | v_false :
@@ -85,14 +88,16 @@ Fixpoint subst (x : string) (s : tm) (t : tm) : tm :=
   match t with
   | tm_var y =>
       if String.eqb x y then s else t
-  | <{\y:T, t1}> =>
-      if String.eqb x y then t else <{\y:T, [x:=s] t1}>
+  | <{\y:ty, t1}> =>
+      if String.eqb x y then t else <{\y:ty, [x:=s] t1}>
   | <{t1 t2}> =>
       <{[x:=s] t1 [x:=s] t2}>
   | <{true}> =>
       <{true}>
   | <{false}> =>
       <{false}>
+  | <{OOPS}> =>
+      <{OOPS}>
   (* | <{if t1 then t2 else t3}> =>
       <{if [x:=s] t1 then [x:=s] t2 else [x:=s] t3}> *)
   end
@@ -107,35 +112,35 @@ Notation "x '|->' v " := ((x, v) :: nil)
 
 Notation "'empty'" := nil (in custom stlc_tm) : stlc_scope.
 
-Reserved Notation "<{ Γ '⊢' t '∈' T }>"
-            (at level 0, Γ custom stlc_tm at level 200, t custom stlc_tm, T custom stlc_ty).
+Reserved Notation "<{ Γ '⊢' t '∈' ty }>"
+            (at level 0, Γ custom stlc_tm at level 200, t custom stlc_tm, ty custom stlc_ty).
 
 Inductive has_type : context -> tm -> ty -> Prop :=
-  | T_Var : forall Γ x T1,
-      lookup Γ x = Some T1 ->
-      <{Γ ⊢ x ∈ T1 }>
-  | T_Abs : forall Γ x T1 T2 t1,
-      <{ x |-> T2 ; Γ ⊢ t1 ∈ T1 }> ->
-      <{ Γ ⊢ \x:T2, t1 ∈ T2 -> T1 }>
-  | T_App : forall T1 T2 Γ t1 t2,
-      <{ Γ ⊢ t1 ∈ T2 -> T1 }> ->
-      <{ Γ ⊢ t2 ∈ T2 }> ->
-      <{ Γ ⊢ t1 t2 ∈ T1 }>
+  | T_Var : forall Γ x ty,
+      lookup Γ x = Some ty ->
+      <{Γ ⊢ x ∈ ty }>
+  | T_Abs : forall Γ x ty1 ty2 t1,
+      <{ x |-> ty2 ; Γ ⊢ t1 ∈ ty1 }> ->
+      <{ Γ ⊢ \x:ty2, t1 ∈ ty2 -> ty1 }>
+  | T_App : forall ty1 ty2 Γ t1 t2,
+      <{ Γ ⊢ t1 ∈ ty2 -> ty1 }> ->
+      <{ Γ ⊢ t2 ∈ ty2 }> ->
+      <{ Γ ⊢ t1 t2 ∈ ty1 }>
   | T_True : forall Γ,
       <{ Γ ⊢ true ∈ Bool }>
   | T_False : forall Γ,
       <{ Γ ⊢ false ∈ Bool }>
-  (* | T_If : forall t1 t2 t3 T1 Γ,
+  (* | T_If : forall t1 t2 t3 ty1 Γ,
        <{ Γ ⊢ t1 ∈ Bool }> ->
-       <{ Γ ⊢ t2 ∈ T1 }> ->
-       <{ Γ ⊢ t3 ∈ T1 }> ->
-       <{ Γ ⊢ if t1 then t2 else t3 ∈ T1 }> *)
+       <{ Γ ⊢ t2 ∈ ty1 }> ->
+       <{ Γ ⊢ t3 ∈ ty1 }> ->
+       <{ Γ ⊢ if t1 then t2 else t3 ∈ ty1 }> *)
 
-where "<{ Γ '⊢' t '∈' T }>" := (has_type Γ t T) : stlc_scope.
+where "<{ Γ '⊢' t '∈' ty }>" := (has_type Γ t ty) : stlc_scope.
 
 Hint Constructors has_type : core.
 
-Definition typable (t : tm) := exists T, <{nil ⊢ t ∈ T}>.
+Definition typable (t : tm) := exists ty, <{nil ⊢ t ∈ ty}>.
 
 Reserved Notation "s '==>' t" (at level 90, left associativity).
 
@@ -143,8 +148,9 @@ Inductive eval : tm -> tm -> Prop :=
   | E_Val : forall v,
     value v ->
     eval v v
-  | E_App : forall t1 t2 x T b v2 v,
-    t1 ==> <{\x : T, b}> ->
+  | E_App : forall t1 t2 x ty b v2 v,
+    ty <> Ty_ERROR ->
+    t1 ==> <{\x : ty, b}> ->
     t2 ==> v2 ->
     <{[x := v2] b}> ==> v ->
     <{t1 t2}> ==> v
@@ -161,53 +167,231 @@ where "s '==>' t" := (eval s t).
 
 Hint Constructors eval : core.
 
-Fixpoint get_type ty : PIR.ty :=
+From MetaCoq.Utils Require Import utils.
+Import MCMonadNotation.
+
+Fixpoint translate_type ty : option PIR.ty :=
   match ty with
-  | Ty_Bool => PIR.Ty_Builtin DefaultUniBool
-  | Ty_Arrow ty1 ty2 => PIR.Ty_Fun (get_type ty1) (get_type ty2) end.
+  | Ty_Bool => Some (PIR.Ty_Builtin DefaultUniBool)
+  | Ty_Arrow ty1 ty2 => 
+      ty1' <- translate_type ty1 ;;
+      ty2' <- translate_type ty2 ;;
+      Some (PIR.Ty_Fun ty1' ty2') 
+  | Ty_ERROR => None end.
 
-Fixpoint translate tm : term :=
+Fixpoint translate tm : option term :=
   match tm with
-  | tm_var x => Var x
-  | tm_app tm1 tm2 => Apply (translate tm1) (translate tm2)
-  | tm_abs x T b => let ty := get_type T in LamAbs x ty (translate b)
-  | tm_true => (Constant (ValueOf DefaultUniBool true))
-  | tm_false => (Constant (ValueOf DefaultUniBool false))
+  | tm_var x => Some (Var x)
+  | tm_app tm1 tm2 => 
+    tm1' <- translate tm1 ;;
+    tm2' <- translate tm2 ;;
+    Some (Apply tm1' tm2')
+  | tm_abs x ty b => 
+    ty' <- translate_type ty ;; 
+    b' <- translate b ;;
+    Some (LamAbs x ty' b')
+  | tm_true => Some (Constant (ValueOf DefaultUniBool true))
+  | tm_false => Some (Constant (ValueOf DefaultUniBool false))
+  | tm_oops => None
   (* | tm_if tm1 tm2 tm3 => Apply (Builtin IfThenElse) t1 *) end.
-
-Notation k := <{ \x:Bool, \y:Bool, x }>.
-
-Eval cbv in (translate k).
 
 Ltac solve_pir_eval := split; [(eexists ; eauto using BigStepPIR.eval) | constructor].
 
-Theorem translate_id_correct : forall v,
-  eval v v ->
-  value v ->
-  evaluatesTo (translate v) (translate v).
+Lemma tl_lambda : forall x ty b t',
+  translate <{\x : ty, b}> = Some t' ->
+  exists b' ty',
+    translate_type ty = Some ty' /\
+    translate b = Some b' /\
+    LamAbs x ty' b' = t'.
 Proof.
-  intros v ev vv. induction vv; solve_pir_eval.
+  intros x ty b t' tl_t.
+  inversion tl_t as [Ht].
+  destruct (translate_type ty) as [ty'|]; try discriminate.
+  destruct (translate b) as [b'|]; try discriminate.
+  inversion Ht as [Ht'].
+  exists b'. exists ty'. auto.
 Qed.
 
-Lemma subst_same : forall x v b,
-  translate <{ [x := v] b }> = BigStepPIR.subst x (translate v) (translate b).
+Lemma tl_lambda' : forall x ty b ty' b',
+  translate_type ty = Some ty' ->
+  translate b = Some b' ->
+  translate <{\x:ty, b}> = Some (LamAbs x ty' b').
 Proof.
-  intros x v b. induction b; simpl.
-  - destruct (x =? s)%string; auto.
-  - rewrite IHb1, IHb2. auto.
-  - destruct (x =? s)%string; auto.
-    simpl. rewrite IHb. auto.
-  - auto.
-  - auto.
+  intros. simpl. rewrite H, H0. reflexivity.
 Qed.
 
-Theorem translate_correct : forall t v,
+Lemma tl_app : forall t1 t2 t',
+  translate <{t1 t2}> = Some t' ->
+  exists t1' t2',
+    translate t1 = Some t1' /\
+    translate t2 = Some t2' /\
+    Apply t1' t2' = t'.
+Proof.
+  intros t1 t2 t' tl_t. inversion tl_t as [Ht].
+  destruct (translate t1) as [t1'|]; try discriminate.
+  destruct (translate t2) as [t2'|]; try discriminate.
+  inversion Ht.
+  exists t1'. exists t2'. auto.
+Qed.
+
+Lemma tl_app' : forall t1 t2 t1' t2',
+  translate t1 = Some t1' ->
+  translate t2 = Some t2' ->
+  translate <{t1 t2}> = Some (Apply t1' t2').
+Proof.
+  intros t1 t2 t1' t2' tl_t1 tl_t2.
+  simpl. rewrite tl_t1. rewrite tl_t2.
+  reflexivity.
+Qed.
+
+Lemma subst_same : forall x v b v' b',
+  translate v = Some v' ->
+  translate b = Some b' ->
+  translate <{[x := v] b}> = Some (BigStepPIR.subst x v' b').
+Proof.
+  intros x v b.
+  induction b; intros v' b' tl_v tl_b.
+  - inversion tl_b. simpl in *. 
+    destruct (x =? s)%string; auto.
+  - apply tl_app in tl_b.
+    destruct tl_b as [t1' [t2' [tl_t1 [tl_t2 eqt]]]].
+    subst. simpl.
+    rewrite (IHb1 v' t1' tl_v tl_t1).
+    rewrite (IHb2 v' t2' tl_v tl_t2).
+    reflexivity.
+  - apply tl_lambda in tl_b.
+    destruct tl_b as [b'' [ty' [tl_ty [tl_b eqb]]]]. 
+    subst. simpl. destruct (x =? s)%string.
+    + simpl. rewrite tl_ty, tl_b. reflexivity.
+    + simpl. rewrite tl_ty. rewrite (IHb v' b'' tl_v tl_b).
+      reflexivity.
+  - inversion tl_b. auto.
+  - inversion tl_b. auto.
+  - discriminate.
+Qed.
+
+Theorem translate_correct : forall t v t',
   eval t v ->
-  exists k, BigStepPIR.eval (translate t) (translate v) k.
+  translate t = Some t' ->
+  exists v' k,
+    translate v = Some v' /\
+    BigStepPIR.eval t' v' k.
+Proof with (eauto using BigStepPIR.eval).
+  intros t v t' ev. revert t'. 
+  induction ev. intros t' tl_t.
+  - destruct H. 
+    + apply tl_lambda in tl_t.
+      destruct tl_t as [b' [ty' [tl_ty [tl_b eq_b]]]].
+      eexists. eexists. split.
+      * simpl. rewrite tl_ty, tl_b. reflexivity.
+      * rewrite <- eq_b...
+    + inversion tl_t. simpl...
+    + inversion tl_t. simpl...
+    - intros ta' tl_ta. apply tl_app in tl_ta.
+    destruct tl_ta as [t1' [t2' [tl_t1 [tl_t2 tl_a]]]].
+    destruct (IHev1 t1' tl_t1) as [lv' [k1 [tl_l step1]]].
+    destruct (IHev2 t2' tl_t2) as [v2' [k2 [tl_v2 step2]]].
+    apply tl_lambda in tl_l.
+    destruct tl_l as [b' [ty' [tl_ty [tl_b eq_b]]]].
+    assert (Hs: translate <{ [x0 := v2] b }> = Some (BigStepPIR.subst x0 v2' b')).
+    apply (subst_same x0 v2 b v2' b' tl_v2 tl_b).
+    destruct (IHev3 (BigStepPIR.subst x0 v2' b') Hs) as [v' [k3 [tl_v step3]]].
+    exists v'. exists (k1 + k2 + 1 + k3). split. apply tl_v. subst.
+    eapply E_Apply. eauto. apply step1. apply step2. apply step3.
+Qed.
+
+Inductive translatesTypeTo : ty -> PIR.ty -> Prop :=
+  | tlty_bool  : translatesTypeTo Ty_Bool (PIR.Ty_Builtin DefaultUniBool)
+  | tlty_arrow : forall ty1 ty2 ty1' ty2',
+      translatesTypeTo ty1 ty1' ->
+      translatesTypeTo ty2 ty2' ->
+      translatesTypeTo (Ty_Arrow ty1 ty2) (PIR.Ty_Fun ty1' ty2').
+
+Inductive translatesTo : tm -> term -> Prop :=
+  | tlt_var : forall x, translatesTo (tm_var x) (Var x)
+  | tlt_app : forall t1 t2 t1' t2', 
+      translatesTo t1 t1' ->
+      translatesTo t2 t2' ->
+      translatesTo (tm_app t1 t2) (Apply t1' t2')
+  | tlt_abs : forall x ty b ty' b', translatesTo b b' ->
+      translatesTypeTo ty ty' ->
+      translatesTo (tm_abs x ty b) (LamAbs x ty' b') 
+  | tlt_true : translatesTo tm_true (Constant (ValueOf DefaultUniBool true))
+  | tlt_false : translatesTo tm_false (Constant (ValueOf DefaultUniBool false)).
+
+Theorem translate_type_reflect : forall ty ty',
+  translate_type ty = Some ty' <-> translatesTypeTo ty ty'.
 Proof.
-  intros t v ev. induction ev.
-  - eexists. induction H; (eauto using BigStepPIR.eval).
-  - simpl in *. destruct IHev1, IHev2, IHev3. eexists.
-    eapply E_Apply with (j1 := x1) (j2 := x2) (j0 := x3). eauto.
-    apply H. apply H0. rewrite <- subst_same. apply H1.
+  intros ty ty'; split.
+  - revert ty'. induction ty; intros ty' tl_ty.
+    + inversion tl_ty. apply tlty_bool.
+    + inversion tl_ty as [Hty].
+      destruct (translate_type ty1) as [ty1'|]; try discriminate.
+      destruct (translate_type ty2) as [ty2'|]; try discriminate.
+      specialize (IHty1 ty1' eq_refl).
+      specialize (IHty2 ty2' eq_refl).
+      inversion Hty as [Hty']. 
+      apply (tlty_arrow ty1 ty2 ty1' ty2' IHty1 IHty2).
+    + discriminate.
+  - intros tl_ty. induction tl_ty.
+    + auto.
+    + simpl. rewrite IHtl_ty1, IHtl_ty2. reflexivity.
+Qed.  
+
+Theorem translate_reflect : forall t t',
+  translate t = Some t' <-> translatesTo t t'.
+Proof. 
+  split.
+  - revert t'. induction t; intros t' tl_t.
+    + inversion tl_t. apply (tlt_var s).
+    + apply tl_app in tl_t.
+      destruct tl_t as [t1' [t2' [tl_t1 [tl_t2 eqt]]]].
+      specialize (IHt1 t1' tl_t1).
+      specialize (IHt2 t2' tl_t2).
+      rewrite <- eqt.
+      apply (tlt_app t1 t2 t1' t2' IHt1 IHt2).
+    + apply tl_lambda in tl_t.
+      destruct tl_t as [b' [ty' [tl_ty [tl_b eq_l]]]].
+      rewrite <- eq_l.
+      apply (tlt_abs s t t0 ty' b' (IHt b' tl_b)).
+      apply translate_type_reflect in tl_ty. apply tl_ty.
+    + inversion tl_t. apply tlt_true.
+    + inversion tl_t. apply tlt_false.
+    + discriminate.
+  - intros tlt_t. induction tlt_t.
+    + auto.
+    + apply tl_app'.
+      apply IHtlt_t1. apply IHtlt_t2.
+    + apply tl_lambda'. apply translate_type_reflect in H.
+      apply H. apply IHtlt_t.
+    + auto.
+    + auto.
+Qed.
+
+Theorem translatesTo_correct : forall t v t',
+  eval t v ->
+  translatesTo t t' ->
+  exists v' k,
+    translatesTo v v' /\
+    BigStepPIR.eval t' v' k.
+Proof with (eauto using BigStepPIR.eval).
+  intros t v t' ev. revert t'.
+  induction ev. intros t' tlt_t.
+  - induction H; inversion tlt_t; exists t'; eexists.
+    + split; [apply tlt_t| subst; eauto using BigStepPIR.eval].
+    + split; [apply tlt_t| subst; eauto using BigStepPIR.eval].
+    + split; [apply tlt_t| subst; eauto using BigStepPIR.eval].
+  - intros t' tlt_t.
+    inversion tlt_t. subst.
+    destruct (IHev1 t1' H2) as [lv' [k1 [tlt_l ev_l]]].
+    destruct (IHev2 t2' H4) as [v2' [k2 [tlt_v2 ev_v2]]].
+    inversion tlt_l.
+    assert (Hs: translate <{ [x0 := v2] b }> = Some (BigStepPIR.subst x0 v2' b')).
+    apply translate_reflect in tlt_v2 as tl_v2.
+    apply translate_reflect in H6 as tl_b.
+    apply (subst_same x0 v2 b v2' b' tl_v2 tl_b).
+    apply translate_reflect in Hs as tlt_s.
+    destruct (IHev3 (BigStepPIR.subst x0 v2' b') tlt_s) as [v' [k3 [tlt_v ev_v]]].
+    exists v'. exists (k1 + k2 + 1 + k3). split. apply tlt_v.
+    eapply E_Apply. eauto. rewrite <- H3 in ev_l. apply ev_l. apply ev_v2. apply ev_v.
 Qed.
