theories/Translation.v
@@ -14,6 +14,7 @@ Local Open Scope string_scope.
 
 Import Kernames ListNotations.
 Import MCMonadNotation.
+Import BasicAst EAst.
 
 Notation "'bs_to_s' s" := (bytestring.String.to_string s) (at level 200).
 Notation "'s_to_bs' s" := (bytestring.String.of_string s) (at level 200).
@@ -33,8 +34,10 @@ Definition remap_env : env PIR.ty :=
 Definition remap_fun (kn : kername) (df : PIR.DefaultFun) :=
   (kn, PIR.Builtin df).
 
-Import BasicAst EAst.
 
+Section translate.
+
+Context (TT : env PIR.ty).
 (* TODO: extend with context to get fresh variable names *)
 (* Definition get_name (na : name) : string :=
   match na with
@@ -42,7 +45,7 @@ Import BasicAst EAst.
   | nNamed nm => if nm =? "_" then "a" else nm
   end. *)
 
-Definition translate_ty (TT : env PIR.ty) : box_type -> option PIR.ty :=
+Definition translate_ty : box_type -> option PIR.ty :=
   fix go (ty : box_type) :=
   match ty with
   | TBox => Some (PIR.Ty_Builtin (PIR.DefaultUniUnit))
@@ -56,40 +59,36 @@ Definition translate_ty (TT : env PIR.ty) : box_type -> option PIR.ty :=
 
 (* proof that welltyped => some t *)
 (* use var approach of malf? *)
-Fixpoint translate_term (TT : env PIR.ty) (ctx : context) (t : term) 
+Fixpoint translate_term (ctx : list bs) (t : term) 
                         {struct t} : annots box_type t -> option PIR.term :=
   match t return annots box_type t -> option PIR.term with
   | tBox => fun b_ty => Some (PIR.Constant (ValueOf DefaultUniUnit tt)) (* temporary constant *)
   | tRel n => fun b_ty =>
     match nth_error ctx n with
-    | Some {| decl_name := na |} =>
-      match na with
-      | nAnon => None (* Anonymous names*)
-      | nNamed id => Some (PIR.Var id)
-      end
+    | Some id => Some (PIR.Var id)
     | None => None
     end
   | tLambda (nNamed x) t => fun '(ty, t_ty) =>
       match ty with
       | TArr a _ =>
-        a' <- translate_ty TT a ;;
-        t' <- translate_term TT (vass (nNamed (s_to_bs x)) :: ctx) t t_ty ;;
+        a' <- translate_ty a ;;
+        t' <- translate_term (x :: ctx) t t_ty ;;
         Some (LamAbs x a' t')
       | _ => None
       end
   | tApp s t => fun '(_, (s_ty, t_ty)) => (* does not handle all arguments yet, eta expansion?*)
-    s' <- translate_term TT ctx s s_ty ;;
-    t' <- translate_term TT ctx t t_ty ;;
+    s' <- translate_term ctx s s_ty ;;
+    t' <- translate_term ctx t t_ty ;;
     Some (PIR.Apply s' t')
   | _ => fun _ => None
   end.
 
-Lemma unfold_lamAbs TT ctx x t ty t_ty :
-  translate_term TT ctx (tLambda (nNamed x) t) (ty, t_ty) = 
+Lemma unfold_lamAbs ctx x t ty t_ty :
+  translate_term ctx (tLambda (nNamed x) t) (ty, t_ty) = 
   match ty with
   | TArr a _ =>
-    a' <- translate_ty TT a ;;
-    t' <- translate_term TT (vass (nNamed (s_to_bs x)) :: ctx) t t_ty ;;
+    a' <- translate_ty a ;;
+    t' <- translate_term (x :: ctx) t t_ty ;;
     Some (LamAbs x a' t')
   | _ => None
   end.
@@ -97,20 +96,103 @@ Proof.
   auto.
 Qed.
 
-Lemma unfold_app TT ctx s t s_ty t_ty res_ty s' t' : 
-  translate_term TT ctx s s_ty = Some s' ->
-  translate_term TT ctx t t_ty = Some t' ->
-  translate_term TT ctx (tApp s t) (res_ty, (s_ty, t_ty)) = Some (PIR.Apply s' t').
+Lemma unfold_app ctx s t s_ty t_ty res_ty s' t' : 
+  translate_term ctx s s_ty = Some s' ->
+  translate_term ctx t t_ty = Some t' ->
+  translate_term ctx (tApp s t) (res_ty, (s_ty, t_ty)) = Some (PIR.Apply s' t').
 Proof.
   intros. simpl. now rewrite H, H0.
 Qed.
 
+Inductive translatesTypeTo : box_type -> PIR.ty -> Prop :=
+  | tlty_tt  : translatesTypeTo TBox (PIR.Ty_Builtin DefaultUniUnit)
+  | tlty_fun : forall ty1 ty2 ty1' ty2',
+      translatesTypeTo ty1 ty1' ->
+      translatesTypeTo ty2 ty2' ->
+      translatesTypeTo (TArr ty1 ty2) (PIR.Ty_Fun ty1' ty2')
+  | tlty_kn  : forall kn ty',
+      lookup TT (string_of_kername kn) = Some ty' ->
+      translatesTypeTo (TConst kn) ty'.
+
+Print box_type.
+Print annots.
+Inductive translatesTo (ctx : list bs) : forall (t : term),
+  annots box_type t -> PIR.term -> Prop :=
+  | tlt_tt : forall ann, translatesTo ctx tBox ann (Constant (ValueOf DefaultUniUnit tt))
+  | tlt_rel : forall n x ann, (* look at rel ordering *)
+      nth_error ctx n = Some x ->
+      translatesTo ctx (tRel n) ann (Var x)
+  | tlt_lambda : forall x ty1 ty2 b ann_b ty1' b',
+      translatesTypeTo ty1 ty1' ->
+      translatesTo (x :: ctx) b ann_b b' ->
+      translatesTo ctx (tLambda (nNamed x) b) ((TArr ty1 ty2), ann_b) (LamAbs x ty1' b')
+  | tlt_app : forall t1 t2 t1' t2' ann_t1 ann_t2 ty,
+      translatesTo ctx t1 ann_t1 t1' ->
+      translatesTo ctx t2 ann_t2 t2' ->
+      translatesTo ctx (tApp t1 t2) (ty, (ann_t1, ann_t2)) (PIR.Apply t1' t2').
+
+Theorem translate_type_reflect : forall ty ty',
+  translate_ty ty = Some ty' <-> translatesTypeTo ty ty'.
+Proof.
+  intros ty ty'; split.
+  - revert ty'. induction ty; try discriminate; intros ty' tl_ty.
+    + inversion tl_ty. apply tlty_tt. 
+    + inversion tl_ty as [Hty].
+      destruct (translate_ty ty1) as [ty1'|]; try discriminate.
+      destruct (translate_ty ty2) as [ty2'|]; try discriminate.
+      specialize (IHty1 ty1' eq_refl).
+      specialize (IHty2 ty2' eq_refl).
+      inversion Hty as [Hty'].
+      apply (tlty_fun ty1 ty2 ty1' ty2' IHty1 IHty2).
+    + inversion tl_ty as [Hl].
+      apply tlty_kn. apply Hl.
+  - intros tl_ty. induction tl_ty.
+    + auto.
+    + simpl. rewrite IHtl_ty1, IHtl_ty2. reflexivity.
+    + auto.
+Qed.
+
+Theorem translate_reflect : forall ctx t t' (ann : annots box_type t),
+  translate_term ctx t ann = Some t' <-> translatesTo ctx t ann t'.
+Proof.
+  split.
+  - revert ctx t'. induction t; try discriminate; intros ctx t' tl_t.
+    + inversion tl_t. apply tlt_tt.
+    + inversion tl_t as [Ht].
+      destruct (nth_error ctx n) eqn:El; try discriminate.
+      inversion Ht as [Ht'].
+      apply tlt_rel. apply El.
+    + inversion tl_t as [Ht]. destruct na; try discriminate.
+      destruct ann as [[] ann_b]; try discriminate.
+      destruct (translate_ty dom) as [ty1'|] eqn:tl_ty; try discriminate.
+      destruct (translate_term (i :: ctx) t ann_b) as [b'|] eqn:tl_b; try discriminate.
+      inversion Ht as [Ht']. subst.
+      specialize (IHt ann_b (i :: ctx) b' tl_b).
+      apply (translate_type_reflect dom ty1') in tl_ty.
+      apply (tlt_lambda ctx i dom codom t ann_b ty1' b' tl_ty IHt).
+    + inversion tl_t as [Ht].
+      destruct ann as [ty [ann_t1 ann_t2]].
+      destruct (translate_term ctx t1 ann_t1) as [t1'|] eqn:tl_t1; try discriminate.
+      destruct (translate_term ctx t2 ann_t2) as [t2'|] eqn:tl_t2; try discriminate.
+      inversion Ht as [Ht'].
+      specialize (IHt1 ann_t1 ctx t1' tl_t1).
+      specialize (IHt2 ann_t2 ctx t2' tl_t2).
+      apply (tlt_app ctx t1 t2 t1' t2' ann_t1 ann_t2 ty IHt1 IHt2).
+  - intros tl_t. induction tl_t.
+    + auto.
+    + simpl. rewrite H. reflexivity.
+    + simpl. apply translate_type_reflect in H. rewrite H.
+      simpl. setoid_rewrite IHtl_t. reflexivity.
+    + simpl. rewrite IHtl_t1, IHtl_t2. reflexivity.
+Qed.
+
+End translate.
+
 Definition translate_unsafe ctx (t : term) (ann : annots box_type t) := 
-  with_default (PIR.Error (PIR.UNDEFINED "TranslationFailed")) ((translate_term remap_env ctx t) ann).
+  with_default (PIR.Error (PIR.UNDEFINED "TranslationFailed")) (translate_term remap_env ctx t ann).
 
 (* Lambda Box T is the combination of an EAst term with a dependent tree of its types
   For now, we pass manual annotations until I set up a proper pipeline *)
-
 Definition identity_EAst : term :=
   tLambda (nNamed (s_to_bs "y")) 
     (tRel 0).
